concurrency/main.v
@@ -1,62 +1,12 @@
 Require Import VST.concurrency.main_definitions.
 Require Import VST.concurrency.compiler.sequential_compiler_correct.
 Require Import VST.concurrency.compiler.concurrent_compiler_simulation_definitions.
+Import Memory.Mem.
 
-
-Module MainTheorem_statement
-       (CC_correct: CompCert_correctness)
-       (Args: ThreadSimulationArguments).
-  Import CC_correct Args.
-  
-  Definition top2bottom_safety: Prop:=
-    (* C program is proven to be safe in CSL*)
-      CSL_correct C_program ->
-
-      (* C program compiles to some assembly program*)
-      forall (asm_prog:Asm.program),
-      CompCert_compiler C_program = Some asm_prog ->
-      
-      forall (src_m:Memory.mem) (src_cpm:Clight.state),
-        (* Initial State for CSL *)
-        CSL_init_setup C_program src_m src_cpm ->
-        
-        (*Correct entry point Clight (There is inconsistencies with CSL_init_Setup)*)
-        (* TODO: fix initial state inconsistenciees and unify. *)
-        Clight.entry_point (Clight.globalenv C_program) src_m src_cpm (main_ptr C_program) nil ->
-        
-        (* ASM memory good. *)
-        forall (limited_builtins:Asm_core.safe_genv x86_context.X86Context.the_ge),
-        asm_prog_well_formed asm_prog limited_builtins ->
-        
-        forall U, exists tgt_m0 tgt_m tgt_cpm,
-            (* inital asm machine *)
-            barebones_init_machine
-              asm_prog limited_builtins
-              tgt_m0 tgt_cpm tgt_m (main_ptr C_program) nil /\
-
-            (*it's spinlock safe: well synchronized and safe *)
-            spinlock_safe U tgt_cpm tgt_m.
-End MainTheorem_statement.
-
+(*PROOFs*)
 Require Import VST.concurrency.main_proofs.
-Require Import VST.concurrency.lib.tactics.
 
-Module MainTheorem_Proof
-       (CC_correct: CompCert_correctness)
-       (Args: ThreadSimulationArguments).
-  Import CC_correct Args.
-  Module Theorem_statement:=MainTheorem_statement CC_correct Args.
-  Module Theorem_proofs:=Main CC_correct Args.
-  Import Theorem_statement Theorem_proofs.
 
-  Hint Unfold top2bottom_safety.
-  Hint Transparent top2bottom_safety.
-  Theorem top2bottom_safety_proof: top2bottom_safety.
-  Proof. (autounfold; eapply main_safety_clean). Qed.
-  
-End MainTheorem_Proof.
-
-(* Test an instantiation of Main theorem. *)
 Module CC_correct: CompCert_correctness.
   Axiom CompCert_compiler : Clight.program -> option Asm.program.
   Axiom simpl_clight_semantic_preservation :
@@ -76,10 +26,78 @@ Module ProgramArgs: ThreadSimulationArguments.
     
 End ProgramArgs.
 
+Module MainTheorem
+       (CC_correct: CompCert_correctness)
+       (Args: ThreadSimulationArguments).
+  Import CC_correct Args.
+  Module Theorem_proofs:=Main CC_correct Args.
+  Import Theorem_proofs.
+  
 
-Module Test_Main:= (MainTheorem_Proof CC_correct ProgramArgs).
+  (* Temporary lemma for exposition. Deleete until ["Delete until here"]*)
+  Import Clight.
+  
+  (* We want to prove something like this. Maybe with extra assumptions, 
+     or (probably) the convers. In the end we want to unify the two predicates. *)
+  Lemma entry_point_problem:
+    forall src_m src_cpm1 src_cpm2,
+      Clight.entry_point
+        (Clight.globalenv C_program) src_m src_cpm1 (main_ptr C_program) nil ->
+      CSL_init_setup C_program src_m src_cpm2 -> src_cpm1 = src_cpm2.
+  Proof.
+    intros * H1  H2.
+    inversion H1; inversion H2; subst.
+    unfold Clight_init_state; simpl.
+    (* The two ways of getting an initial state:
+         LHS -  Clight_init_state, how the CSL proof defines initial states
+         RHS -  Clight.entry_point our new way of defining initial states 
+                (entry points)
+     *)
+    rename f into f_main2.
+    destruct f_main2.
+    - admit.
+    - 
+    
+    - admit. (* initial states don't match. *)
+  Admitted.
+      
+
+      (* End of temporary exposition *)
+  Goal True.
+    idtac "Delete until here". auto. Qed.
+
+  Theorem top2bottom_correct:
+    (* C program is proven to be safe in CSL*)
+      CSL_correct C_program ->
+
+      (* C program compiles to some assembly program*)
+      CompCert_compiler C_program = Some Asm_program ->
+      
+      forall (src_m:Memory.mem) (src_cpm:Clight.state),
+        (* Initial State for CSL *)
+        CSL_init_setup C_program src_m src_cpm ->
+        
+        (*Correct entry point Clight (There is inconsistencies with CSL_init_Setup)*)
+        (* TODO: fix initial state inconsistenciees and unify. *)
+        Clight.entry_point (Clight.globalenv C_program) src_m src_cpm (main_ptr C_program) nil ->
+        
+        (* ASM memory good. *)
+        forall (limited_builtins:Asm_core.safe_genv x86_context.X86Context.the_ge),
+        asm_prog_well_formed Asm_program limited_builtins ->
+        
+        forall (U:schedule), exists (tgt_m0 tgt_m: mem) (tgt_cpm:ThreadPool.t),
+            (* inital asm machine *)
+            permissionless_init_machine
+              Asm_program limited_builtins
+              tgt_m0 tgt_cpm tgt_m (main_ptr C_program) nil /\
+
+            (*it's spinlock safe: well synchronized and safe *)
+            spinlock_safe U tgt_cpm tgt_m.
+    Proof. eapply main_safety_clean. Qed.
+End MainTheorem.
+
+Module Test_Main:= (MainTheorem CC_correct ProgramArgs).
 Import Test_Main.
 
-Check Theorem_statement.top2bottom_safety.
-Check top2bottom_safety_proof.
-Print Assumptions top2bottom_safety_proof.
+Check top2bottom_correct.
+Print Assumptions top2bottom_correct.
